io/case-studies/case-study-2/WebServer.Compiled.fst
@@ -11,42 +11,9 @@ open Shared
 open TC.MLify.MIIO
 open WebServer
 
-let extract_local_trace (h':trace) (pi:monitorable_prop) :
-  IIO trace pi
-    (requires (fun h -> h' `suffix_of` h))
-    (ensures (fun h lt' lt ->
-      lt == [] /\
-      h == (apply_changes h' lt'))) =
-  let h = get_trace () in
-  suffix_of_length h' h;
-  let n : nat = (List.length h) - (List.length h') in
-  let (lt', ht) = List.Tot.Base.splitAt n h in
-  lemma_splitAt_equal n h;
-  lemma_splitAt_suffix h h';
-  List.Tot.Properties.rev_involutive lt';
-  assert (h == apply_changes h' (List.rev lt'));
-  List.rev lt'
-
-let enforce_post
-  (#i:interface)
-  (#pi:monitorable_prop)
-  (f:i.ctx_arg -> IIO (maybe i.ctx_ret) pi (fun _ -> True) (fun _ _ _ -> true))
-  (x:i.ctx_arg) :
-  IIO (maybe i.ctx_ret) pi (fun _ -> True) (i.ctx_post x)  =
-  let h = get_trace () in
-  let r : maybe i.ctx_ret = f x in
-  Classical.forall_intro (lemma_suffixOf_append h);
-  let lt = extract_local_trace h pi in
-  Classical.forall_intro_2 (Classical.move_requires_2 (lemma_append_equals h));
-  if i.ctx_post_c.check4 x h r lt then r
-  else Inr Contract_failure
-
 let compiled_webserver : prog_t i pi = comp.compile_prog #i #pi webserver
-val compiled_webserver' : (file_descr -> Tot (maybe unit)) -> MIIO (maybe unit)
-let compiled_webserver' f = compiled_webserver (enforce_post #i #pi f)
-
 let compiled_webserver'' : (Types.file_descr -> Tot (maybe unit)) -> ML (maybe unit) = 
   mlify
     #((Types.file_descr -> Tot (maybe unit)) -> MIIO (maybe unit))
     #(mlifyable_tot_miio file_descr (maybe unit) (maybe unit) #TC.Export.ml_file_descr)
-    compiled_webserver'
+    compiled_webserver
